Aus der Definition
$$ \ddot\theta_1 = \frac{1}{1 - \mu \cos(\theta_2 - \theta_1)} \cdot \mu g_1 \sin(\theta_2) \cos(\theta_2 - \theta_1) + \mu \dot\theta_1^2 \sin(\theta_2 - \theta_1) \cos(\theta_2 - \theta_1) - g_1 \sin(\theta_2) - \lambda \dot\theta_2^2 \sin(\theta_2 - \theta_1) $$
wird mit $\theta_1 \approx \theta_2 \approx 0$
$$ \Rightarrow \dot\theta_i^2 = 0, $$
und
$$ \cos(\theta_2 - \theta_1) = 1 $$
also ist
$$ \ddot\theta_1 = \frac{\mu g_1 \sin(\theta_2) - g_1 \sin(\theta_1)}{1 - \mu} $$
